ArkLib/OracleReduction/Basic.lean
@@ -4,7 +4,7 @@ Released under Apache 2.0 license as described in the file LICENSE.
 Authors: Quang Dao
 -/
 
-import ArkLib.OracleReduction.ProtocolSpec.Basic
+import ArkLib.OracleReduction.ProtocolSpec.SeqCompose
 
 /-!
 # Interactive (Oracle) Reductions
